compiler/backend/word_instScript.sml
@@ -45,44 +45,124 @@ val flatten_exp_def = tDefine "flatten_exp" `
 
 (*val test = EVAL ``flatten_exp (Op Add [Const 1w;Const 2w; Const 3w; Op Add [Const 4w; Const 5w; Op Add[Const 6w; Const 7w]] ; Const 8w])``*)
 
-(* Next, perform instruction selection assuming input is binary branching
+(*
+  Maximal Munch instruction selection on (binary) expressions
+  c is an asm_config to check validity of imms (TODO: assume 0w is accepted?)
+  Implemented (optimized) munches (assumes Consts are sorted to the front):
+  Load [Op Add [Const w;exp]]
+  Op op [Const w; exp]
+  Store exp var
+
+  Next, perform instruction selection assuming input is binary branching
   Each step takes tar and temp where we are allowed to store temporaries 
   in temp and the value of the whole expression must be saved in tar
 *)
 val inst_select_exp_def = tDefine "inst_select_exp" `
-  (*TODO: Add special cases so we never need to reach this case*)
-  (inst_select_exp (tar:num) (temp:num) (Const w) = (Inst (Const tar w))) ∧
-  (inst_select_exp (tar:num) (temp:num) (Var v) =
-    Move 0 [tar,v]) ∧
-  (inst_select_exp tar temp (Lookup store_name) = 
-    Get tar store_name) ∧ 
-  (*For Load, flatten the expression into a temp
-    Can be improved (by matching an offset in the nested exp)
-  *)
-  (inst_select_exp tar temp (Load exp) = 
-    let prog = inst_select_exp temp temp exp in
+  (*TODO: Reduce the ugly amount of case splitting?*)
+  (inst_select_exp (c:'a asm_config) (tar:num) (temp:num) (Load (Op Add [Const w;exp])) =
+    let prog = inst_select_exp c temp temp exp in
+      if addr_offset_ok w c 
+      then 
+        Seq prog (Inst (Mem Load tar (Addr temp w)))
+      else if c.valid_imm (INL Add) w
+      then
+        let prog' = Inst (Arith (Binop Add temp temp (Imm w))) in
+        let prog'' = Inst (Mem Load tar (Addr temp 0w)) in
+        Seq prog (Seq prog' prog'')
+      else
+        let prog' = Inst (Const (temp+1) w) in
+        let prog'' = Inst (Arith (Binop Add temp temp (Reg (temp+1)))) in
+        let prog''' = Inst (Mem Load tar (Addr temp 0w)) in
+        Seq prog (Seq prog' (Seq prog'' prog'''))) ∧
+   (inst_select_exp c tar temp (Load exp) = 
+    let prog = inst_select_exp c temp temp exp in
     Seq prog (Inst (Mem Load tar (Addr temp (0w))))) ∧ 
+  (inst_select_exp c (tar:num) (temp:num) (Const w) = (Inst (Const tar w))) ∧
+  (inst_select_exp c (tar:num) (temp:num) (Var v) =
+    Move 0 [tar,v]) ∧
+  (inst_select_exp c tar temp (Lookup store_name) = 
+    Get tar store_name) ∧ 
   (*All ops are binary branching*)
-  (inst_select_exp tar temp (Op op [e1;e2]) =
-    let p1 = inst_select_exp temp temp e1 in
-    let p2 = inst_select_exp (temp+1) (temp+1) e2 in
-    Seq p1 (Seq p2 ((Inst (Arith (Binop op tar temp (Reg (temp+1)))))))) ∧ 
-  (inst_select_exp tar temp (Shift sh exp nexp) =
-    let prog = inst_select_exp temp temp exp in
+  (inst_select_exp c tar temp (Op op [Const w;e2]) = 
+    let p2 = inst_select_exp c (temp+1) (temp+1) e2 in
+    if c.valid_imm (INL op) w then
+      Seq p2 (Inst (Arith (Binop op tar temp (Imm w))))
+    else
+      let p1 = Inst (Const temp w) in
+      Seq p1 (Seq p2 (Inst (Arith (Binop op tar temp (Reg (temp+1))))))) ∧
+  (inst_select_exp c tar temp (Op op [e1;e2]) =
+    let p1 = inst_select_exp c temp temp e1 in
+    let p2 = inst_select_exp c (temp+1) (temp+1) e2 in
+    Seq p1 (Seq p2 (Inst (Arith (Binop op tar temp (Reg (temp+1))))))) ∧ 
+  (inst_select_exp c tar temp (Shift sh exp nexp) =
+    let prog = inst_select_exp c temp temp exp in
     (*nexp should be evaluated at compile time*) 
     let n = num_exp nexp in 
     Seq prog (Inst (Arith (Shift sh tar temp n)))) ∧ 
   (*Make it total*)
-  (inst_select_exp _ _ _ = Skip)`
-  (WF_REL_TAC `measure (exp_size ARB o SND o SND)`
+  (inst_select_exp _ _ _ _ = Skip)`
+  (WF_REL_TAC `measure (exp_size ARB o SND o SND o SND)`
    \\ REPEAT STRIP_TAC \\ IMP_RES_TAC MEM_IMP_exp_size
    \\ TRY (FIRST_X_ASSUM (ASSUME_TAC o Q.SPEC `ARB`))
    \\ fs[exp_size_def]
    \\ TRY (DECIDE_TAC)) ;
 (*
-EVAL ``inst_select_exp 0 1 (Op And [Op Add [Var 2;Var 3; Var 4]; Const 0w; Const 0w])``
+
+First munch
+EVAL ``inst_select_exp x64_config 5 5 (Load (Op Add [Const 400w; Var 6]))``
+EVAL ``inst_select_exp x64_config 5 5 (Load (Op Add [Const 99999999999w; Var 6]))``
+
+Second munch
+EVAL ``inst_select_exp x64_config 0 99 (Op And [Const 99w;Op Add [Var 2;Var 3]])``
+
 *)
 
+(*Flattens all expressions in program, temp must a fresh var*)
+val inst_select_def = Define`
+  (inst_select c temp (Assign v exp) = 
+    (inst_select_exp c v temp o flatten_exp) exp) ∧ 
+  (inst_select c temp (Set store exp) =
+    let prog = (inst_select_exp c temp temp o flatten_exp) exp in
+    Seq prog (Set store (Var temp))) ∧
+  (inst_select c temp (Store exp var) =
+    let exp = flatten_exp exp in
+    case exp of 
+    | Op Add [Const w;exp] =>
+      let prog = inst_select_exp c temp temp exp in
+      if addr_offset_ok w c 
+      then 
+        Seq prog (Inst (Mem Store var (Addr temp w)))
+      else if c.valid_imm (INL Add) w
+      then
+        let prog' = Inst (Arith (Binop Add temp temp (Imm w))) in
+        let prog'' = Inst (Mem Store var (Addr temp 0w)) in
+        Seq prog (Seq prog' prog'')
+      else
+        let prog' = Inst (Const (temp+1) w) in
+        let prog'' = Inst (Arith (Binop Add temp temp (Reg (temp+1)))) in
+        let prog''' = Inst (Mem Store var (Addr temp 0w)) in
+        Seq prog (Seq prog' (Seq prog'' prog'''))
+        
+    | _ => 
+      let prog = inst_select_exp c temp temp exp in
+        Seq prog (Inst (Mem Store var (Addr temp 0w)))) ∧ 
+  (inst_select c temp (Seq p1 p2) =
+    Seq (inst_select c temp p1) (inst_select c temp p2)) ∧ 
+  (inst_select c temp (If cmp r1 ri c1 c2) =
+    If cmp r1 ri (inst_select c temp c1) (inst_select c temp c2)) ∧ 
+  (inst_select c temp (Call ret dest args handler) =
+    let retsel =
+      case ret of 
+        NONE => NONE
+      | SOME (n,names,ret_handler,l1,l2) =>
+        SOME (n,names,inst_select c temp ret_handler,l1,l2) in
+    let handlersel = 
+      case handler of
+        NONE => NONE
+      | SOME (n,h,l1,l2) => SOME (n,inst_select c temp h,l1,l2) in
+    Call retsel dest args handlersel) ∧ 
+  (inst_select c temp prog = prog)`
+  
 (*
   Convert all 3 register instructions to 2 register instructions
 *)
@@ -108,34 +188,6 @@ val three_to_two_reg_def = Define`
     Call retsel dest args handlersel) ∧ 
   (three_to_two_reg prog = prog)`
 
-(*Flattens all expressions in program, temporary must a fresh var*)
-val inst_select_def = Define`
-  (inst_select temp (Assign v exp) = 
-    (inst_select_exp v temp o flatten_exp) exp) ∧ 
-  (inst_select temp (Set store exp) =
-    let prog = (inst_select_exp temp temp o flatten_exp) exp in
-    Seq prog (Set store (Var temp))) ∧
-  (*Can be optimised further*) 
-  (inst_select temp (Store exp var) =
-    let prog = (inst_select_exp temp temp o flatten_exp) exp in
-    Seq prog (Inst (Mem Store var (Addr temp 0w)))) ∧ 
-  (inst_select temp (Seq p1 p2) =
-    Seq (inst_select temp p1) (inst_select temp p2)) ∧ 
-  (inst_select temp (If cmp r1 ri c1 c2) =
-    If cmp r1 ri (inst_select temp c1) (inst_select temp c2)) ∧ 
-  (inst_select temp (Call ret dest args handler) =
-    let retsel =
-      case ret of 
-        NONE => NONE
-      | SOME (n,names,ret_handler,l1,l2) =>
-        SOME (n,names,inst_select temp ret_handler,l1,l2) in
-    let handlersel = 
-      case handler of
-        NONE => NONE
-      | SOME (n,h,l1,l2) => SOME (n,inst_select temp h,l1,l2) in
-    Call retsel dest args handlersel) ∧ 
-  (inst_select temp prog = prog)`
-  
 val _ = export_theory();
 
 
